implemented all handlers except load & store

Programs.v
@@ -7,6 +7,7 @@ Definition z :=3.
 Definition a :=1.
 Definition b :=2.
 Definition c :=3.
+Definition t0 :=0.
 Definition t1 :=1.
 Definition t2 :=2.
 Definition l1 :=1.
@@ -30,22 +31,22 @@ Definition p1_t2 (l : lock):=
     Unlock l
 ].
 
-Definition p1 :=
+Definition p1 t1 t2:=
 [
     Spawn t1 (p1_t1 l1);
     Spawn t2 (p1_t2 l1);
-    Wait(t1);
-    Wait(t2)
+    Wait t1;
+    Wait t2
 ].
 
 (* a racy program*)
 
-Definition p2 :=
+Definition p2 t1 t2:=
 [
     Spawn t1 (p1_t1 l1);
     Spawn t2 (p1_t2 l2);  (* x is protected by different locks*)
-    Wait(t1);
-    Wait(t2)
+    Wait t1;
+    Wait t2
 ].
 
 (*Definition handler (cop : conc_op):=
@@ -73,26 +74,67 @@ Definition inc_vc t tgt tmp := [
   Store (tgt, t) (V tmp)
 ].
 
+Fixpoint max_vc tgt src z tmp1 tmp2 :=
+match z with
+| 0 => []
+| S n => [
+    Load tmp1 (src,n); 
+    Load tmp2 (tgt,n);
+    Assign tmp2 (Max (V tmp1) (V tmp2));
+    Store (tgt,n) (V tmp2)
+]++ max_vc tgt src n tmp1 tmp2
+end.
+
+
+
+(* TODO: load & store handlers*)
 (* Since everything is a nat, we can use C + t as the t component of C. *)
-Definition load_handler t x C R tmp := move (C + t, t) (R + x, t) tmp.
-
+Definition load_handler t x C R (W : var) tmp := move (C + t, t) (R + x, t) tmp.
+Definition store_handler t x C (R:var) W tmp := move (C + t, t) (W + x, t) tmp.
+Definition lock_handler t l C L z tmp1 tmp2 :=
+  max_vc (C+t) (L+l) z tmp1 tmp2.
+  
 Definition unlock_handler t l (C : var (* start of thread VCs *))
-  (L : var (* start of lock VCs *)) z tmp :=
-  set_vc (L + l) (C + t) z tmp ++ inc_vc t (C + t) tmp.
-
+  (L : var (* start of lock VCs *)) z tmp1 tmp2 :=
+  max_vc (L + l) (C + t) z tmp1 tmp2 ++ inc_vc t (C + t) tmp1.
+Definition spawn_handler t a C z tmp :=
+  set_vc (C + a) (C + t) z tmp ++ inc_vc t (C + t) tmp.
+Definition wait_handler t a C z tmp1 tmp2 :=
+  max_vc (C + t) (C + a) z tmp1 tmp2.
 (* The instrumentation pass is provided locations to store each of the
    race detection state components. *)
-Definition instrument_instr (C L R W : var) z tmp (ins : instr) (t : tid)
+Definition instrument_instr (C L R W : var) z tmp1 tmp2 (ins : instr) (t : tid)
   : prog :=
 (match ins with
- | Load a (x, 0)   => load_handler t x C R tmp
- (* | ... *)
- | Unlock l   => unlock_handler t l C L z tmp
- | _          => []
-end) ++ [ins].
+ | Load a (x, 0)   => load_handler t x C R W tmp1 ++ [ins]
+ | Store (x, 0) e  => store_handler t x C R W tmp1 ++ [ins]
+ | Lock l          =>  lock_handler t l C L z tmp1 tmp2 ++ [ins]
+ | Unlock l   => unlock_handler t l C L z tmp1 tmp2 ++ [ins]
+ | Spawn a li =>  spawn_handler t a C z tmp1 ++ [ins] 
+ | Wait a     => [ins] ++ wait_handler t a C z tmp1 tmp2  (* the wait_handler should be called after the wait returns*)
+ | _          => [ins]
+end).
 
-Fixpoint instrument C L R W z tmp (p: prog) (t: tid) : prog:=
+Fixpoint instrument C L R W z tmp1 tmp2 (p: prog) (t: tid) : prog:=
 match p with
 | [] => []
-| ins::inss => (instrument_instr C L R W z tmp ins t)++(instrument C L R W z tmp inss t)
+| ins::inss => (instrument_instr C L R W z tmp1 tmp2 ins t)++(instrument C L R W z tmp1 tmp2 inss t)
 end.
+
+Definition C_base := 16.
+Definition L_base := 32.
+Definition R_base := 48.
+Definition W_base := 64.
+Definition local_base := 0.
+
+Definition instrumented_p1 :=instrument C_base L_base R_base W_base 3 local_base (local_base+1) (p1 1 2) t0.
+Definition instrumented_p1_t1 := instrument C_base L_base R_base W_base 3 local_base (local_base+1) (p1_t1 l1) t1.
+Definition instrumented_p1_t2 := instrument C_base L_base R_base W_base 3 local_base (local_base+1) (p1_t2 l1) t2.
+
+Theorem dummy: instrumented_p1 = instrumented_p1.
+Proof.
+  unfold instrumented_p1,t0.
+  simpl.
+  
+  reflexivity.
+Qed.
